\section{Exercice 4}

On a \[
	\begin{cases}
		a_{n+1} = \frac{1}{2} b_n + \frac{1}{2} c_n\\
		b_{n+1} = \frac{1}{2} a_n + \frac{1}{2} c_n\\
		c_{n+1} = \frac{1}{2} a_n + \frac{1}{2} b_n.\\
	\end{cases}
\]
D'où, \[
	\underbrace{\begin{pmatrix}
		a_{n+1}\\b_{n+1}\\c_{n+1}
	\end{pmatrix}}_{U_{n+1}} = \frac{1}{2} \underbrace{\begin{pmatrix}
		0&1&1\\
		1&0&1\\
		1&1&0
	\end{pmatrix}}_M \cdot \underbrace{\begin{pmatrix}
		a_{n}\\b_{n}\\c_{n}
	\end{pmatrix}}_{U_n}
.\]
Diagonalisons cette matrice $M$.
On a \[
	\chi_M(X) = (X - 1)^2 \cdot (X + 2)
.\]
En effet, soit $\lambda \in \R$, on calcule
\begin{align*}
	\det(\lambda I_3 - M) &=
	\begin{vmatrix}
		\lambda & -1 & -1\\
		-1 & \lambda & -1\\
		-1 & -1 & \lambda
	\end{vmatrix}\\
	&= 
	\begin{vmatrix}
		\lambda + 1 & -\lambda - 1 & 0\\
		0 & \lambda + 1 & -\lambda- 1\\
		-1 & -1 & \lambda
	\end{vmatrix}\\
	&= (\lambda + 1) \left( 
	\begin{vmatrix}
		\lambda + 1 & -\lambda - 1\\
		-1 & \lambda
	\end{vmatrix} + 
	\begin{vmatrix}
		0 & -\lambda - 1\\
		-1 & \lambda
	\end{vmatrix}\right) \\
	&= (\lambda + 1)(\lambda^2 + \cancel\lambda - \cancel\lambda - 1 - \lambda - 1)\\
	&= (\lambda + 1)(\lambda^2 - \lambda + 2) \\
	&= (\lambda + 1)^2\cdot (\lambda - 2) \\
\end{align*}

D'où, $\Sp(M) = \{1,-2\}$.


